theories/CTree/Logic/Trans.v
@@ -46,11 +46,14 @@ Section CTreeTrans.
       trans tau t t' ->
       not_done w ->
       ktrans_ (t, w) (t', w)
-    | KtransDone (x: X) (t t': ctree E X) w:
+    | KtransDone (x: X) (t t': ctree E X):
       trans (val x) t stuck ->
       t' ≅ stuck ->
-      not_done w ->
-      ktrans_ (t, w) (t', Done x).
+      ktrans_ (t, Pure) (t', Done x)
+    | KtransFinish (e: E) (v: encode e) (x: X) (t t': ctree E X):
+      trans (val x) t stuck ->
+      t' ≅ stuck ->
+      ktrans_ (t, Obs e v) (t', Finish e v x).      
   
   Global Instance trans_equ_proper:
     Proper (equ eq * eq ==> equ eq * eq ==> iff) ktrans_.
@@ -64,9 +67,15 @@ Section CTreeTrans.
     - apply KtransDone; auto.
       + now rewrite <- Heqt.
       + now rewrite <- Heqt0.
+    - apply KtransFinish; auto.
+      + now rewrite <- Heqt.
+      + now rewrite <- Heqt0.
     - apply KtransObs; auto. now rewrite Heqt0, Heqt.
     - apply KtransTau; auto. now rewrite Heqt0, Heqt.
     - apply KtransDone; auto.
+      + now rewrite Heqt.
+      + now rewrite Heqt0.
+    - apply KtransFinish; auto.
       + now rewrite Heqt.
       + now rewrite Heqt0.
   Qed.
@@ -75,42 +84,48 @@ Section CTreeTrans.
   Lemma ktrans_trans: forall t t' w w',
       ktrans_ (t, w) (t', w') <->
         (exists l, trans_ l (observe t) (observe t') /\
-                not_done w /\
-                ((l = tau /\ w' = w)
-                 \/ (exists e (x: encode e), l = obs e x /\ w' = Obs e x)
-                 \/ (exists (x: X), l = val x /\ t' ≅ stuck /\ w' = Done x))).
+                ((l = tau /\ not_done w /\ w' = w)
+                 \/ (exists e (x: encode e), l = obs e x /\ not_done w /\ w' = Obs e x)
+                 \/ (exists (x: X), l = val x /\ w = Pure /\ t' ≅ stuck /\ w' = Done x)
+                 \/ (exists e (v: encode e) (x: X), l = val x /\ w = Obs e v /\ t' ≅ stuck /\ w' = Finish e v x))).
   Proof.
     intros; split; intro H.    
     - inv H. 
-      + exists (obs e x); split; auto; split; auto.
+      + exists (obs e x); split; auto. 
         right; left.
         exists e, x; auto.
       + exists tau; split; auto.
-      + exists (val x); rewrite H5; split; auto; split; auto with ctl.
-        right; right.
+      + exists (val x); rewrite H5; split; auto.
+        right; right; left.
         exists x; auto.
-    - destruct H as (l & ? & ? & []).
-      + destruct H1 as (-> & ->).
+      + exists (val x); rewrite H5; split; auto.
+        right; right; right.
+        exists e, v, x; auto.
+    - destruct H as (l & ? & []).
+      + destruct H0 as (-> & ? & ->).
         now apply KtransTau.
-      + destruct H1 as [(e & x & -> & ->) | (x & -> & ? & ->)].
+      + destruct H0 as [(e & x & -> & ? & ->) | [(x & -> & -> & ? & ->) | (e & v & x & -> & -> & ? & ->)]].
         * now apply KtransObs.
-        * rewrite H1 in *.
+        * rewrite H0 in *.
           apply KtransDone; auto with trans.
+        * rewrite H0 in *.
+          apply KtransFinish; auto with trans.
   Qed.
 
 End CTreeTrans.
 
 Ltac ktrans_inv H :=
-  let Hw := fresh "Heqw" in
   let e := fresh "e" in
   let x := fresh "x" in
   let v := fresh "v" in
   let l := fresh "l" in
   let Ht := fresh "Heqt" in
   apply ktrans_trans in H as
-        (l & H & ? & [(Hl & Hw) |
-                        [(e & x & Hl & Hw) |
-                          (x & Hl & Ht & Hw) ]]); subst.
+        (l & H &
+           [ (? & ? & ?) |
+             [(e & x & ? & ? & ?) |
+               [(x & ? & ? & Ht & ?) |
+                 (e & v & x & ? & ? & Ht & ?)]]]); subst.
 
 Global Hint Constructors ktrans_: core.
 
@@ -130,59 +145,52 @@ Section CTreeTrans.
     + split; [apply KtransTau|]; auto.      
     + split; [apply KtransObs|]; auto.
     + split; auto.
-      pose proof trans_val_inv H2.
-      rewrite <- H4 in *.
+      pose proof trans_val_inv H1.
+      rewrite <- H3 in *.
       now apply KtransDone.
+    + split; auto.
+      pose proof trans_val_inv H1.
+      rewrite <- H3 in *.
+      now apply KtransFinish.
   Defined.
   Next Obligation.
     ktrans_inv H; auto with ctl; inv H0.
   Defined.
   Next Obligation.
-    ktrans_inv H; apply H0; auto. 
+    ktrans_inv H; auto with ctl. 
   Defined.
 
   (*| Lemmas that depend on structure of [ctrees] |*)
   Lemma ktrans_brD {X}: forall n (t': ctree E X) (k: fin' n -> ctree E X) w w',
-      (BrD n k, w) ↦ (t', w') <->
-        (exists (i: fin' n), (k i, w) ↦ (t', w')).
+      ktrans_ (BrD n k, w) (t', w') <->
+        (exists (i: fin' n), ktrans_ (k i, w) (t', w')).
   Proof.
     split; intro H.
     - ktrans_inv H; apply trans_brD_inv in H as (n' & ?);
         exists n'; apply ktrans_trans; eexists.
-      + split; [eassumption|split]; auto. 
-      + split; [eassumption|split]; auto.
-        right; left; eauto.
-      + split; [eassumption|split]; auto.
-        right; right.
-        exists x; auto.
+      + split; [eassumption|]; left; auto.
+      + split; [eassumption|]; right; left; eauto.
+      + split; [eassumption|]; right; right; left; eauto.
+      + split; [eassumption|]; right; right; right; exists e, v, x; auto.
     - destruct H as (n' & H); ktrans_inv H; apply ktrans_trans; eexists.
-      + split; [|split].
-        * econstructor; eassumption.
-        * assumption.
-        * left; split; reflexivity. 
-      + split; [|split].
-        * econstructor; eassumption.
-        * assumption.
-        * right; left; exists e, x; split; reflexivity.
-      + split; [|split].
-        * econstructor; eassumption.
-        * assumption.
-        * right; right; exists x; split; auto.
+      + split; [econstructor|left]; eauto.
+      + split; [econstructor|right; left]; eauto.
+      + split; [econstructor|right; right; left]; eauto.
+      + split; [econstructor; apply H|right; right; right];exists e, v, x; eauto.
   Qed.
 
   Lemma ktrans_brS {X}: forall n (t: ctree E X) (k: fin' n -> ctree E X) w w',
-      (BrS n k, w) ↦ (t, w') <->
+      ktrans_ (BrS n k, w) (t, w') <->
         (exists (i: fin' n), t ≅ k i /\ w = w' /\ not_done w).
   Proof.
     split; intro H.
     - ktrans_inv H; apply trans_brS_inv in H as (n' & ? & ?);
-        exists n'; subst; inv H1; auto.
+        exists n'; subst; inv H0; auto.
     - destruct H as (n' & -> & -> & ?).
       apply ktrans_trans; exists tau.
       split; econstructor.
       * reflexivity.
       * auto.
-      * now left.
   Qed.
   
   Lemma ktrans_guard {X}: forall (t t': ctree E X) s s',
@@ -193,12 +201,20 @@ Section CTreeTrans.
     - apply ktrans_brD; now (exists (F1)).
   Qed.
 
-  Lemma ktrans_ret {X}: forall (t: ctree E X) (w w': World E) (e: E) (v: encode e) x,
-      ktrans_ (Ret x, w) (t, w') <-> (not_done w /\ w' = Done x /\ t ≅ stuck).
+  Lemma ktrans_pure {X}: forall (t: ctree E X) (w': World E) x,
+      ktrans_ (Ret x, Pure) (t, w') <-> (w' = Done x /\ t ≅ stuck).
   Proof.
     intros; split; intros.
-    - ktrans_inv H; dependent destruction H; split; auto.
-    - destruct H as (? & -> & ->); etrans. 
+    - ktrans_inv H; dependent destruction H; split; auto with ctl.
+    - destruct H as (-> & ->); etrans. 
+  Qed.
+
+  Lemma ktrans_finish {X}: forall (t: ctree E X) (w': World E) (e: E) (v: encode e) x,
+      ktrans_ (Ret x, Obs e v) (t, w') <-> (w' = Finish e v x /\ t ≅ stuck).
+  Proof.
+    intros; split; intros.
+    - ktrans_inv H; dependent destruction H; split; auto with ctl.
+    - destruct H as (-> & ->); etrans. 
   Qed.
 
   Lemma ktrans_vis{X}: forall (t: ctree E X) (s s': World E) (e: E) (k: encode e -> ctree E X),
@@ -214,19 +230,20 @@ Section CTreeTrans.
         * step; step in H; cbn in *; rewrite <- x; auto.
         * assumption.
       + inv TR.
+      + inv TR.
     - destruct TR as (? & -> & <- & ?).
       apply ktrans_trans; exists (obs e x).
-      split; [econstructor|split]; auto.
+      split; [econstructor|]; auto.      
       right; left; eauto.
   Qed.
 
-  Lemma ktrans_pure{X}: forall (t t': ctree E X) w,
+  Lemma ktrans_pure_pred{X}: forall (t t': ctree E X) w,
       ktrans_ (t, w) (t', Pure) -> w = Pure.
   Proof.
     intros * H.
     inv H; reflexivity.
   Qed.
-  Hint Resolve ktrans_pure: ctl.
+  Hint Resolve ktrans_pure_pred: ctl.
   
   Lemma ktrans_not_done{X}: forall (t t': ctree E X) w w',
     (t, w) ↦ (t', w') -> not_done w.
@@ -245,57 +262,98 @@ Section CTreeTrans.
     - exists tau; split. (* BrS *)
       + apply trans_bind_l; auto.
         intro Hcontra; inv Hcontra.
-      + split; auto with ctl.
+      + left; auto with ctl.
     - exists (obs e x); split. (* Vis *)
       + apply trans_bind_l; auto.
         intro Hcontra; inv Hcontra; world_inv.
-      + split; auto with ctl. (* Ret *)
-        right; eauto.
+      + auto with ctl. (* Ret *)
+        right; left; eauto.      
+    - inv H0.
     - inv H0.
   Qed.
 
-  Lemma ktrans_bind_r{X Y}: forall (t: ctree E Y) (u: ctree E X) (k: Y -> ctree E X) (y: Y) w w',
-      ktrans_ (t, w) (stuck, Done y) ->
+  Lemma ktrans_bind_r{X Y}: forall (t: ctree E Y) (u: ctree E X) (k: Y -> ctree E X) (y: Y) w w_ w',
+      ktrans_ (t, w) (stuck, w_) ->
+      is_done_with w_ y ->
       ktrans_ (k y, w) (u, w') ->
       ktrans_ (y <- t ;; k y, w) (u, w').
   Proof.
     intros.
-    ktrans_inv H; apply ktrans_trans; try world_inv.
-    - inv H1. 
-    - ktrans_inv H0. 
+    ktrans_inv H; apply ktrans_trans; try world_inv; dependent destruction H0.
+    - inv H3.
+    - inv H3.
+    - ktrans_inv H1. 
       + exists tau; split.
         * apply trans_bind_r with x; auto.          
-        * split; auto.
+        * left; auto. 
       + exists (obs e x0); split.
         * apply trans_bind_r with x; etrans.
-        * split; auto.
-          right; left; eauto.
+        * right; left; eauto. 
       + exists (val x0); split.
         * apply trans_bind_r with x; etrans.
-        * split; auto.
-          right; right; eauto.
+        * right; right; left; eauto.
+      + inv H2.
+    - ktrans_inv H1; try world_inv.
+      + exists tau; split.
+        * apply trans_bind_r with x; auto.          
+        * left; auto. 
+      + exists (obs e0 x0); split.
+        * apply trans_bind_r with x; etrans.
+        * right; left; eauto. 
+      + exists (val x0); split.
+        * apply trans_bind_r with x; etrans.
+        * right; right; right; exists e0, v0, x0; etrans.
   Qed.
 
-  Lemma ktrans_bind_inv{X Y}: forall (t: ctree E Y) (u: ctree E X) (k: Y -> ctree E X) (w w': @World E HE) ,
+  Lemma ktrans_bind_inv{X Y}: forall (t: ctree E Y) (u: ctree E X) (k: Y -> ctree E X) (w w': World E) ,
       ktrans_ (x <- t ;; k x, w) (u, w') ->
       (exists t', ktrans_ (t, w) (t', w')
              /\ not_done w'
              /\ u ≅ x <- t' ;; k x) \/
       (exists y, ktrans_ (t, w) (stuck, Done y)
-            /\ ktrans_ (k y, w) (u, w')).
+             /\ w = Pure /\ ktrans_ (k y, w) (u, w')) \/
+      (exists (e: E) (v: encode e) y, ktrans_ (t, w) (stuck, Finish e v y)
+             /\ w = Obs e v /\ ktrans_ (k y, w) (u, w')).
   Proof.
     intros * TR.
     ktrans_inv TR; destruct (trans_bind_inv _ _ TR) as
-      [(Hv & t' & TR' & Heq) | (y & TRv & TR')]. 
+      [(Hv & t' & TR' & Heq) | (y & TRv & TR')].
     - left; exists t'; split; auto.
-    - right; exists y; split; auto; apply ktrans_trans.
+    - inv H0.
+      + right; left; exists y; split; [apply ktrans_trans|split]; auto with ctl.
+        exists (val y); split; auto.
+        right; right; left; exists y; auto.
+      + right; right; exists e, v, y; split; auto with ctl.       
     - left; exists t'; split; auto with ctl.
-    - right; exists y; split; auto; apply ktrans_trans.
+    - inv H0.
+      + right; left; exists y; split; [apply ktrans_trans|split]; auto with ctl.
+        exists (val y); split; auto.
+        right; right; left; exists y; auto.
+      + right; right; exists e0, v, y; split; auto with ctl.
     - exfalso; apply Hv; constructor.
-    - right; exists y; split; auto; apply ktrans_trans.
-      exists (val x); split; [|split]; auto.
-      right; right.
-      exists x; auto.
+    - right; left; exists y; split; [apply ktrans_trans|split]; auto.
+      exists (val y); split; auto with ctl.
+      right; right; left; exists y; auto.
+      rewrite (ctree_eta (k y)) in *; cbn.
+      desobs (k y). apply trans_ret_inv in TR' as (-> & ?); dependent destruction H. 
+      + eauto with trans ctl.
+      + destruct b.
+        inv TR'.
+        rewrite Heqt in *.
+        econstructor; eauto with ctl.
+      + inv TR'.
+    - exfalso; apply Hv; constructor.
+    - right; right; exists e, v, y; split; [apply ktrans_trans|split]; auto.      
+      exists (val y); split; auto with ctl.
+      right; right; right; exists e, v, y; auto.
+      rewrite (ctree_eta (k y)) in *; cbn.
+      desobs (k y). apply trans_ret_inv in TR' as (-> & ?); dependent destruction H. 
+      + eauto with trans ctl.
+      + destruct b.
+        inv TR'.
+        rewrite Heqt in *.
+        econstructor; eauto with ctl.
+      + inv TR'.
   Qed.
 
 End CTreeTrans.
@@ -308,11 +366,13 @@ Proof.
   intros.
   unfold trigger in H3.
   apply ktrans_bind_inv in H3 as
-      [(t' & TR & Hd & Hequ) | (x & TR & Hequ)].
+      [(t' & TR & Hd & Hequ) | [(x & TR & Hequ) | (e' & v & x & TR & -> & Hequ)]].
   - apply ktrans_vis in TR as (y & ? & ? & ?).
     unfold resum, ReSum_refl, resum_ret, ReSumRet_refl in *; world_inv.
     split; [auto | exists y]; split; [reflexivity|].
     now rewrite <- H4, bind_ret_l in Hequ.
   - apply ktrans_vis in TR as (y & ? & ? & ?); world_inv.
+  - split; auto with ctl.
+    apply ktrans_vis in TR as (y & ? & ? & ?); world_inv.
 Qed.
 
